
$$
d(x_i,x_j) = \sum\limits_{k=1}^m (x_{ki}-x_{kj})^2 = {||x_i-x_j||}^2
$$


$ J_e = \sum\limits^k_{i=1}\sum\limits_{y\in \Gamma_i}{||y-m_i||}^2 $



$$ m_i = \dfrac{1}{N} \sum\limits_{y \in \Gamma_i}y $$
$$
S(n,k) = \dfrac{1}{k!} \sum\limits_{l=1}^k(-1)^{k-l}\begin{pmatrix}k \\ l\end{pmatrix}k^n
$$

$$
\overline{m}_c = m_c + \dfrac{1}{N_c-1}[m_c-y]
$$

$$
\overline{m}_j = m_j + \dfrac{1}{N_j-1}[y-m_j]
$$

$$
\tilde{J}_c = J_c - \dfrac{N_c}{N_c-1}{||y-m_c||}^2
$$

$$
\tilde{J}_j = J_j + \dfrac{N_j}{N_j+1}{||y-m_j||}^2
$$

$$
\dfrac{N_j}{N_j+1}{||y-m_j||}^2< \dfrac{N_c}{N_c-1}{||y-m_c||}^2
$$

$$
X = \begin{pmatrix}0&0&1&5&5 \\ 2&0&0&0&2 \end{pmatrix}
$$

